\chapter{3. Image of a clothed black hole}
\pagebreak[4]

\section{General setting}
\begin{figure}[H]
 \centering
\input{./images/fig_Coordinate_system_b.tex}
\caption{General setting.}
\label{fig:fig_4}
\end{figure}
$$\blacklozenge$$\newpage
\section{The coordinate system (enhanced):}

\begin{figure}[H]
 \centering
\input{./images/fig_Coordinate_system.tex}
\caption{The coordinate system (see text).}
\label{fig:fig_3}
\end{figure}
$$\blacklozenge$$\newpage



\section{Angles relationships: equations $(9)$ and $(10)$}

\begin{figure}[H]
 \centering
\input{./images/fig_Coordinate_system_c.tex}
\caption{Different spheric triangles used to find a relation between $\phi,\, \theta_0,\, \alpha$.}
\label{fig:fig_5}
\end{figure}
Resolving the different spherical triangles in order to have a relation between $\phi,\, \theta_0,\, \alpha$.\\
We have (using the basis spherical triangles identities $\frac{\sin{a}}{\sin{A}}= \frac{\sin{b}}{\sin{B}}=\frac{\sin{c}}{\sin{B}}$ and $\cos{a}=\cos{b}\cos{c}+\sin{b}\sin{c}\cos{A}$)\\\\
i) $\Delta Y'_2MY$

\begin{align*}
\frac{\cos{\theta_0}}{\sin{\eta}}&=\frac{\sin{\gamma}}{\sin{\frac{\pi}{2}}}=\frac{\sin{\phi}}{\sin{Y_2}}\\
\cos{(\frac{\pi}{2}-\theta_0)}&=\cos{\gamma}\cos{\phi}+\sin{\gamma}\sin{\phi}\cos{\eta}\\
\cos{\gamma}&=\cos{(\frac{\pi}{2}-\theta_0)}\cos{\phi}+\sin{(\frac{\pi}{2}-\theta_0)}\sin{\phi}\cos{\frac{\pi}{2}}\\
\cos{\phi}&=\cos{\gamma}\cos{(\frac{\pi}{2}-\theta_0)}+\sin{\gamma}\sin{(\frac{\pi}{2}-\theta_0)}\cos{Y'_2}
\end{align*}
ii) $\Delta X'MX_2$
\begin{align*}
\frac{\cos{\alpha}}{\sin{\eta}}&=\frac{\sin{x}}{\sin{X_2}}=\frac{\cos{\phi}}{\sin{X^{'}}}\\
\cos{(\frac{\pi}{2}-\alpha)}&=\cos{(\frac{\pi}{2}-\phi)}\cos{x}+\sin{(\frac{\pi}{2}-\phi)}\sin{x}\cos{\eta}\\
\cos{(\frac{\pi}{2}-\phi)}&=\cos{(\frac{\pi}{2}-\alpha)}\cos{x}+\sin{(\frac{\pi}{2}-\alpha)}\sin{x}\cos{X'}\\
\cos{x}&=\cos{(\frac{\pi}{2}-\alpha)}\cos{(\frac{\pi}{2}-\phi)}+\sin{(\frac{\pi}{2}-\alpha)}\sin{(\frac{\pi}{2}-\phi)}\cos{X_1}
\end{align*}
iii) $\Delta YX_1X'$
\begin{align*}
\frac{\sin{\frac{\pi}{2}}}{\sin{\frac{\pi}{2}}}&=\frac{\cos{\theta_0}}{\sin{X_1}}=\frac{\sin{\frac{\pi}{2}}}{\sin{Y'}}\\
\cos{(\frac{\pi}{2}-\theta_0)}&=\cos{\frac{\pi}{2}}\cos{\frac{\pi}{2}}+\sin{\frac{\pi}{2}}\sin{\frac{\pi}{2}}\cos{X_1}\\
\cos{\frac{\pi}{2}}&=\cos{(\frac{\pi}{2}-\theta_0)}\cos{\frac{\pi}{2}}+\sin{(\frac{\pi}{2}-\theta_0)}\sin{\frac{\pi}{2}}\cos{\frac{\pi}{2}}\\
\cos{\frac{\pi}{2}}&=\cos{\frac{\pi}{2}}\cos{(\frac{\pi}{2}-\theta_0)}+\sin{\frac{\pi}{2}}\sin{(\frac{\pi}{2}-\theta_0)}\cos{Y'}
\end{align*}
iv) $\Delta XY'_1X'$
\begin{align*}
\frac{\cos{\alpha}}{\sin{Y'_1}}&=\frac{\sin{\frac{\pi}{2}}}{\sin{X'}}=\frac{\sin{(x+\gamma)}}{\sin{\frac{\pi}{2}}}\\
\cos{(\frac{\pi}{2}-\alpha)}&=\cos{\frac{\pi}{2}}\cos{(x+\gamma)}+\sin{\frac{\pi}{2}}\sin{(x+\gamma)}\cos{Y'_1}\\
\cos{\frac{\pi}{2}}&=\cos{(x+\gamma)}\cos{(\frac{\pi}{2}-\alpha)}+\sin{(x+\gamma)}\sin{(\frac{\pi}{2}-\alpha)}\cos{X'}\\
\cos{(x+\gamma)}&=\cos{\frac{\pi}{2}}\cos{(\frac{\pi}{2}-\alpha)}+\sin{\frac{\pi}{2}}\sin{(\frac{\pi}{2}-\alpha)}\cos{\frac{\pi}{2}}
\end{align*}
Simplifying:
\begin{align*}
\frac{\cos{\theta_0}}{\sin{\eta}}&=\sin{\gamma}=\frac{\sin{\phi}}{\sin{Y_2}}\\
\frac{\cos{\alpha}}{\sin{\eta}}&=\frac{\sin{x}}{\sin{X_2}}=\frac{\cos{\phi}}{\sin{X^{'}}}\\
\cos{\theta_0}&=\sin{X_1}\\
Y'&=\frac{\pi}{2}\\
\frac{\cos{\alpha}}{\sin{Y'_1}}&=\frac{1}{\sin{X'}}=\sin{(x+\gamma)}\\
\sin{\theta_0}&=\cos{\gamma}\cos{\phi}+\sin{\gamma}\sin{\phi}\cos{\eta}\\
\cos{\gamma}&=\sin{\theta_0}\cos{\phi}\\
\cos{\phi}&=\cos{\gamma}\sin{\theta_0}+\sin{\gamma}\cos{\theta_0}\cos{Y'_2}\\
\sin{\alpha}&=\sin{\phi}\cos{x}+\cos{\phi}\sin{x}\cos{\eta}\\
\sin{\phi}&=\sin{\alpha}\cos{x}+\cos{\alpha}\sin{x}\cos{X'}\\
\cos{x}&=\sin{\alpha}\sin{\phi}+\cos{\alpha}\cos{\phi}\cos{X_1}\\
\sin{\theta_0}&=\cos{X_1}\\
\sin{\alpha}&=\sin{(x+\gamma)}\cos{Y'_1}\\
0&=\cos{(x+\gamma)}\sin{\alpha}+\sin{(x+\gamma)}\cos{\alpha}\cos{X'}\\
0&=\cos{(x+\gamma)}
\end{align*}
and get (discarding all other equation which are not relevant for the problem):
\begin{align}
\frac{\cos{\theta_0}}{\sin{\eta}}&=\sin{\gamma}\\
\frac{\cos{\alpha}}{\sin{\eta}}&=\cos{\phi}\\
\cos{\gamma}&=\sin{\theta_0}\cos{\phi}
\end{align}
From $(1)$ and $(2)$ we get \footnote{In the paper, in equation $(9)$ we see $\cos{\alpha}= \frac{\cot{\phi}\cos{\theta_0}}{\sin{\gamma}}$, which is wrong ($\cot{\phi}$ should be $\cos{\phi})$ as otherwise $\cos{\alpha}$ could become greater than $1$ for certain values of $\phi$.}
\begin{align}\sin{\gamma} =\frac{\cos{\phi}\cos{\theta_0}}{\cos{\alpha}}\end{align} and combining this with $(3)$ we get (squaring both equations and  add them up)
$$\cos{\alpha}= \frac{\cos{\phi}\cos{\theta_0}}{\sqrt{1-\sin^2{\theta_0}\cos^2{\phi}}}$$\\
Equation $(10)$ in the paper follows from equations $(3)$ and $(4)$ by elimination of $\phi$.

$$\blacklozenge$$\newpage
\section{Derivation of equation $(11)$,  $(12)$, $(13)$.}
As can be seen in figure $3.2.$ the photon will reach the plaque (at infinity) after having spanned the angle $\gamma$. Hence,
\begin{align}
\gamma&= \frac{1}{\sqrt{2M}}\int_{0}^{\frac{1}{r}}\frac{dt}{\sqrt{G(t)}}\nonumber \\
&= \underbrace{\frac{1}{\sqrt{2M}}\int_{0}^{\frac{1}{P}}\frac{dt}{\sqrt{G(t)}}}_{2\sqrt{\frac{P}{Q}}\left[K{\left(k\right)}-F{\left(\zeta_{\infty},k\right)}\right]}+\frac{1}{\sqrt{2M}}\int_{\frac{1}{P}}^{\frac{1}{r}}\frac{dt}{\sqrt{G(t)}}\nonumber \\
&=2\sqrt{\frac{P}{Q}}\left[K{\left(k\right)}-F{\left(\zeta_{\infty},k\right)}\right]-\frac{1}{\sqrt{2M}}\int^{\frac{1}{P}}_{\frac{1}{r}}\frac{dt}{\sqrt{G(t)}}
\end{align}
Let's recall equation $(3)$ in section $2.3.$:
\begin{align}
E(z)
&=2\sqrt{2M}\sqrt{\frac{P}{Q}}\int_{\varphi}^{\frac{\pi}{2}}\frac{d\tau}{\sqrt{1-k^{2}\sin^{2}{\left(\tau\right)}}}\quad\quad\small{\left(x=\sin{\left(\tau\right)}\right)}
\end{align}
The upper integration limit $\frac{\pi}{2}$ corresponds to the $\frac{1}{P}$ spherical radial distance, but here for calculating  $\varphi=\arcsin{\left(\sqrt{\frac{z-u_1}{u_2-u_1}}\right)}\in\left(0,\frac{\pi}{2}\right)$ instead of taking $z=0$ as we did previously, we have to take $z=\frac{1}{r}$ which gives 
\begin{align}
\sin^2{\varphi}_{|z=\frac{1}{r}}&=\frac{\frac{1}{r}-u_1}{u_2-u_1}\nonumber \\
&=\frac{\frac{1}{r}+\frac{Q-P+2M}{4MP}}{\frac{1}{P}+\frac{Q-P+2M}{4MP}}\nonumber \\
&=\frac{Q-P+2M+\frac{4MP}{r}}{Q-P+6M}
\end{align}
Let's put \begin{align}\sin^2{\zeta_{r}}=\frac{Q-P+2M+\frac{4MP}{r}}{Q-P+6M}\end{align}\\
$(2)$ becomes
\begin{align}
E(z)
&=2\sqrt{2M}\sqrt{\frac{P}{Q}}\int_{\zeta_{r}}^{\frac{\pi}{2}}\frac{d\tau}{\sqrt{1-k^{2}\sin^{2}{\left(\tau\right)}}}\nonumber \\
&= 2\sqrt{2M}\sqrt{\frac{P}{Q}}\int_{\zeta_{r}}^{0}\frac{d\tau}{\sqrt{1-k^{2}\sin^{2}{\left(\tau\right)}}}+2\sqrt{2M}\sqrt{\frac{P}{Q}}\int_{0}^{\frac{\pi}{2}}\frac{d\tau}{\sqrt{1-k^{2}\sin^{2}{\left(\tau\right)}}}\nonumber \\
&= -2\sqrt{2M}\sqrt{\frac{P}{Q}}\int^{\zeta_{r}}_{0}\frac{d\tau}{\sqrt{1-k^{2}\sin^{2}{\left(\tau\right)}}}+2\sqrt{2M}\sqrt{\frac{P}{Q}}K{\left(k\right)}\nonumber \\
&= -2\sqrt{2M}\sqrt{\frac{P}{Q}}F{\left(\zeta_{r},k\right)}+2\sqrt{2M}\sqrt{\frac{P}{Q}}K{\left(k\right)}
\end{align}
Substituting this in $(1)$:
\begin{align}
\gamma&=2\sqrt{\frac{P}{Q}}\left[K{\left(k\right)}-F{\left(\zeta_{\infty},k\right)}\right]-\frac{1}{\sqrt{2M}}2\sqrt{2M}\sqrt{\frac{P}{Q}}K{\left(k\right)}+\frac{1}{\sqrt{2M}}2\sqrt{2M}\sqrt{\frac{P}{Q}}F{\left(\zeta_{r},k\right)}\nonumber \\
&=2\sqrt{\frac{P}{Q}}\left[K{\left(k\right)}-F{\left(\zeta_{\infty},k\right)}\right]-2\sqrt{\frac{P}{Q}}K{\left(k\right)}+2\sqrt{\frac{P}{Q}}F{\left(\zeta_{r},k\right)}\nonumber \\
&= 2\sqrt{\frac{P}{Q}}\left[F{\left(\zeta_{r},k\right)} -F{\left(\zeta_{\infty},k\right)}\right]
\end{align}
The only term which depends explicitly on $r$ is $F{\left(\zeta_{r},k\right)}$. We rewrite $(5)$ as 
\begin{align}
F{\left(\zeta_{r},k\right)} &= \half \gamma\sqrt{\frac{Q}{P}}+F{\left(\zeta_{\infty},k\right)}
\end{align}

Let $\mathrm{sn}(u,k)$ be the usual Jacobian elliptic function with $ \sin{\zeta_{r}}= \mathrm{sn}(F{\left(\zeta_{r},k\right)})$.\\
We get
\begin{align*}
\sin{\zeta_{r}} &=\mathrm{sn}\left( \half \gamma\sqrt{\frac{Q}{P}}+F{\left(\zeta_{\infty},k\right)}\right)
\end{align*}
From which:
\begin{align}
&\sin^2{\zeta_{r}} =\mathrm{sn}^2\left( \half \gamma\sqrt{\frac{Q}{P}}+F{\left(\zeta_{\infty},k\right)}\right)\nonumber \\
(4)\,\implies\quad &\frac{Q-P+2M+\frac{4MP}{r}}{Q-P+6M} =\mathrm{sn}^2\left( \half \gamma\sqrt{\frac{Q}{P}}+F{\left(\zeta_{\infty},k\right)}\right)\nonumber \\
\implies\quad &\frac{1}{r} =-\frac{Q-P+2M}{4MP}+\frac{Q-P+6M}{4MP}\mathrm{sn}^2\left( \half \gamma\sqrt{\frac{Q}{P}}+F{\left(\zeta_{\infty},k\right)}\right)
\end{align}
Note that in the paper the coefficient $\frac{Q}{P}$ is wrongly written  as $\frac{P}{Q}$
$$\blacklozenge$$\newpage

The derivative of the Jacobi elliptic function $\text{sn}(u, k)$ with respect to the parameter $k$ is given by:

$$
\frac{d}{dk} \text{sn}(u, k) = \text{cn}(u, k) \, \text{dn}(u, k)
$$

Where $\text{cn}(u, k)$ and $\text{dn}(u, k)$ are the Jacobi elliptic functions associated with $\text{sn}(u, k)$.

The derivative of the Jacobi elliptic function $\text{sn}(u, k)$ with respect to the variable $u$ is given by:

$$
\frac{d}{du} \text{sn}(u, k) = \text{cn}(u, k) \, \text{dn}(u, k)
$$

Where $\text{cn}(u, k)$ and $\text{dn}(u, k)$ are the Jacobi elliptic functions associated with $\text{sn}(u, k)$.

The complete elliptic integral of the first kind, denoted as $K(k)$, is a function of the modulus $k$. Since it's not dependent on the variable $u$, its derivative with respect to $u$ is zero:

$$
\frac{d}{du} K(k) = 0
$$

The derivative of the complete elliptic integral of the first kind, $( K(k) )$, with respect to the parameter $( k )$ is given by:

$$[ \frac{dK(k)}{dk} = \frac{E(k)}{k(1-k^2)} ]$$

Where $( E(k) )$ is the complete elliptic integral of the second kind.


The derivative of the incomplete elliptic integral of the first kind, $( F(p, k) )$, with respect to the parameter $( k )$ is not expressible in simple elementary functions. However, it can be represented in terms of the elliptic integrals of the first and second kind and the complete elliptic integral of the first kind.

The derivative is given by:

$$[ \frac{dF(p, k)}{dk} = \frac{\Pi(n, k) - K(k)}{2k(1-k^2)} ]$$

Where $ ( n = 1 - p ), ( K(k) )$ is the complete elliptic integral of the first kind, and $( \Pi(n, k) )$ is the complete elliptic integral of the third kind with modulus $( n )$.

The derivative of the incomplete elliptic integral of the first kind, $( F(p, k) )$, with respect to the parameter $( p )$ is not expressible in simple elementary functions. However, it can be represented in terms of the elliptic integrals of the first and second kind and the complete elliptic integral of the first kind.

The derivative is given by:

$$[ \frac{dF(p, k)}{dp} = \frac{K(k') - E(k')}{2p(1-p)(1-k^2)} ]$$

Where $( k' = \sqrt{1 - k^2} )$,$ ( K(k) )$ is the complete elliptic integral of the first kind, and $( E(k) )$ is the complete elliptic integral of the second kind.